finish the proof on the count example (w/o-table version)

examples/count/verif.v
@@ -4,11 +4,15 @@ Open Scope string_scope.
 
 Import ListNotations.
 Require Import ProD3.examples.count.p4ast.
+(* Require Import Coq.micromega.Lia.
+Require Import Coq.micromega.Nia. *)
+Require Import Psatz.
 
 Require Import Poulet4.Maps.
 Require Import Poulet4.Semantics.
 Require Import Poulet4.SimplExpr.
 Require Import Poulet4.V1Model.
+Require Import Poulet4.P4Arith.
 Require Import ProD3.core.Hoare.
 (* Require Import ProD3.core.AssertionLang. *)
 
@@ -31,7 +35,7 @@ Notation ident := (P4String.t Info).
 Notation path := (list ident).
 Transparent IdentMap.empty IdentMap.set PathMap.empty PathMap.set.
 
-Module Experiment2.
+Module Experiment.
 Definition this : path := [!"main"; !"ig"].
 Definition init_st : state := (PathMap.empty, init_es).
 
@@ -46,22 +50,95 @@ Definition myFundef := Eval compute in
 
 Definition v1 : @ValueBase Info := ValBaseHeader [(!"firstBit", ValBaseBit 1%nat 0)] true.
 Definition v2 : @ValueBase Info := ValBaseStruct [(!"myHeader", v1)].
-Definition v3 : @ValueBase Info := ValBaseStruct [(!"counter", ValBaseBit 4%nat 0)].
-Definition v4 : @ValueBase Info := ValBaseStruct [(!"counter", ValBaseBit 4%nat 1)].
-Definition v5 : @ValueBase Info := ValBaseStruct [(!"egress_spec", ValBaseBit 9%nat 0)].
+Definition v3 : @ValueBase Info := ValBaseStruct [(!"counter", ValBaseBit 4%nat 10)].
+Definition v4 : @ValueBase Info := ValBaseStruct [(!"counter", ValBaseBit 4%nat 0)].
+Definition v5 : @ValueBase Info := ValBaseStruct [(!"egress_spec", ValBaseBit 9%nat 10)].
 Definition v6 : @ValueBase Info := ValBaseStruct [(!"egress_spec", ValBaseBit 9%nat 0)].
 
-Print init_es.
+(* 
+Lemma test: (0 <= P4Arith.BitArith.mod_bound 32 0)%Z.
+Proof.
+  apply Zlt_succ_le.
+  simpl. reflexivity.
+Qed. *)
 
+Ltac Zify.zify_post_hook ::= Z.to_euclidean_division_equations.
 
 (* {st' signal | exec_block [] inst_mem init_st myBlock st' signal }. *)
 Lemma eval_func: { st' & { signal | exec_func ge this inst_m init_st myFundef
     [] [v2; v3; v5] st' [v2; v4; v6] signal} }.
 Proof.
-  repeat econstructor.
-  
-
-
   solve [repeat econstructor].
 Defined.
 
+Opaque IdentMap.empty IdentMap.set PathMap.empty PathMap.set PathMap.sets.
+Definition st'' := Eval compute in (projT1 eval_func).
+
+Definition st' := (PathMap.set (loc_to_path this (LInstance !["meta"]))
+(ValBaseStruct
+   [(!"counter",
+    ValBaseBit
+      (reg_width
+         {| reg_width := 4; reg_size := 2; reg_content := [0; 0] |})
+      (Znth
+         (BitArith.mod_bound (Pos.of_nat 32)
+            (value
+               {| tags := NoInfo; value := 0; width_signed := None |}))
+         (reg_content
+            {| reg_width := 4; reg_size := 2; reg_content := [0; 0] |})))])
+(PathMap.set (loc_to_path this (LInstance !["standard_metadata"]))
+   (ValBaseStruct
+      [(!"egress_spec",
+       ValBaseBit 9
+         (BitArith.mod_bound (Pos.of_nat 9)
+            (value
+               {| tags := NoInfo; value := 0; width_signed := None |})))])
+   (PathMap.sets
+      (filter_in
+         (map (map_fst (fun param : ident => (this ++ [param])%list)) []))
+      (extract_invals [])
+      (PathMap.sets
+         (filter_in
+            (map (map_fst (fun param : ident => (this ++ [param])%list))
+               [(!"hdr", InOut); (!"meta", InOut);
+               (!"standard_metadata", InOut)])) 
+         [v2; v3; v5] PathMap.empty))),
+PathMap.set [!"main"; !"ig"; !"myCounter"]
+(ObjRegister
+  {|
+    reg_width :=
+      reg_width
+        {| reg_width := 4; reg_size := 2; reg_content := [0; 0] |};
+    reg_size :=
+      reg_size
+        {| reg_width := 4; reg_size := 2; reg_content := [0; 0] |};
+    reg_content :=
+      upd_Znth
+        (BitArith.mod_bound (Pos.of_nat 32)
+           (value {| tags := NoInfo; value := 0; width_signed := None |}))
+        (reg_content
+           {| reg_width := 4; reg_size := 2; reg_content := [0; 0] |})
+        (BitArith.plus_mod
+           (Pos.of_nat
+              (reg_width
+                 {|
+                   reg_width := 4; reg_size := 2; reg_content := [0; 0]
+                 |}))
+           (Znth
+              (BitArith.mod_bound (Pos.of_nat 32)
+                 (value
+                    {|
+                      tags := NoInfo; value := 0; width_signed := None
+                    |}))
+              (reg_content
+                 {|
+                   reg_width := 4; reg_size := 2; reg_content := [0; 0]
+                 |}))
+           (BitArith.mod_bound (Pos.of_nat 4)
+              (value
+                 {| tags := NoInfo; value := 1; width_signed := None |})))
+  |}) init_es).
+
+Goal st'' = st'. reflexivity. Qed.
+
+End Experiment.
